{
 "cells": [
  {
   "cell_type": "markdown",
   "id": "f57831b3-9e39-4936-ab62-f844bf8e6a72",
   "metadata": {},
   "source": [
    "**Name:** Raiken Lee D. Ladrera &emsp; **Program & Year:** BSCS - 1\n",
    "\n",
    "---\n",
    "---"
   ]
  },
  {
   "cell_type": "markdown",
   "id": "fe8f8a3f",
   "metadata": {},
   "source": [
    "$\\textbf{1. }$ *Recall the definition of a rational number, denoted as $\\mathbb{Q}$. Prove that the Euler's number $e = \\Sigma_{k=0}^\\infty \\frac{1}{k!} \\notin \\mathbb{Q}$. A factorial is defined as $k! = (k)(k-1)(k-2)(k-3)..., \\forall k \\in \\mathbb{Z}^+$, note that $0! = 1$. Furthermore, a sum notation $\\Sigma_{k=0}^\\infty k = 0+ 1 + 2 + 3 +....+...$*\n",
    "\n",
    "***SOLUTION:***\n",
    "\n",
    "**Step 1:**\n",
    "\n",
    "To prove that Euler's number $e$ is irrational, we'll proceed by contradiction. \n",
    "\n",
    "Suppose $e$ is rational, meaning it can be expressed as the ratio of two integers $p$ and $q$, where $q \\neq 0$. So, $e = \\frac{p}{q}$.\n",
    "\n",
    "**Step 2:**\n",
    "\n",
    "Recall the definition of $ e $ as the sum of the series $ e = \\sum_{k=0}^\\infty \\frac{1}{k!} $. This means:\n",
    "\n",
    "$ e = \\frac{1}{0!} + \\frac{1}{1!} + \\frac{1}{2!} + \\frac{1}{3!} + \\ldots $\n",
    "\n",
    "**Step 3:**\n",
    "\n",
    "Consider the partial sum of the series, denoted as $ S_n $, where $ S_n = \\sum_{k=0}^n \\frac{1}{k!} $ for some positive integer $ n $. Since each term in the series is positive, $ S_n $ is increasing and bounded above by $ e $. Thus, as $ n $ approaches infinity, $ S_n $ converges to $ e $.\n",
    "\n",
    "**Step 4:**\n",
    "\n",
    "Now, consider the number \n",
    "\n",
    "$ q! \\cdot S_n = q! \\cdot \\left(\\frac{1}{0!} + \\frac{1}{1!} + \\frac{1}{2!} + \\frac{1}{3!} + \\ldots + \\frac{1}{n!}\\right) $.\n",
    "\n",
    "**Step 5:**\n",
    "\n",
    "Expand this expression to get \n",
    "\n",
    "$ q! \\cdot S_n = q! + \\frac{q!}{1!} + \\frac{q!}{2!} + \\frac{q!}{3!} + \\ldots + \\frac{q!}{n!} $.\n",
    "\n",
    "**Step 6:**\n",
    "\n",
    "Notice that every term in this expression is an integer. However, since $ S_n $ converges to $ e $, $ q! \\cdot S_n $ should be very close to $ q! \\cdot e = p $. \n",
    "\n",
    "**CONCLUSION**\n",
    "\n",
    "This implies that $ p - q! \\cdot S_n $ should be a very small positive integer. \n",
    "\n",
    "However, $ p - q! \\cdot S_n $ can be expressed as $ (p - q!) - \\frac{q!}{1!} - \\frac{q!}{2!} - \\frac{q!}{3!} - \\ldots - \\frac{q!}{n!} $. \n",
    "\n",
    "Each term in the parentheses is an integer, but each term in the summation is a fraction with the denominator greater than 1.\n",
    "\n",
    "Thus, $ p - q! \\cdot S_n $ cannot be a non-zero positive integer. This contradicts the assumption that $ e $ is rational.\n",
    "\n",
    "Therefore, the initial assumption that $ e $ is rational must be false, and hence $ e $ is **irrational**.\n",
    "\n",
    "---\n",
    "---"
   ]
  },
  {
   "cell_type": "markdown",
   "id": "1aa5adf3",
   "metadata": {},
   "source": [
    "$\\textbf{2. }$ *Prove Minkowski's Inequality for sums, $\\forall \\ p>1, (a_k, b_k)>0$:*\n",
    "\\begin{gather}\n",
    "\\begin{bmatrix}\n",
    "\\Sigma_{k=1}^n |a_k + b_k|^p\n",
    "\\end{bmatrix}^\\frac{1}{p}\n",
    "\\leq\n",
    "\\begin{bmatrix}\n",
    "\\Sigma_{k=1}^n |a_k|^p\n",
    "\\end{bmatrix}^\\frac{1}{p}\n",
    "+\n",
    "\\begin{bmatrix}\n",
    "\\Sigma_{k=1}^n |b_k|^p\n",
    "\\end{bmatrix}^\\frac{1}{p}\n",
    "\\end{gather}.\n",
    "\n",
    "***SOLUTION:***\n",
    "\n",
    "**Step 1:**  \n",
    "\n",
    "First, let's establish the base case for $ n = 1 $.  \n",
    "\n",
    "For $ n = 1 $, the inequality becomes:  \n",
    "\n",
    "$ |a_1 + b_1|^p \\leq |a_1|^p + |b_1|^p $\n",
    "\n",
    "**Step 2:**  \n",
    "\n",
    "Assume the inequality holds for some arbitrary $ n = k $, i.e.,  \n",
    "\n",
    "$ \\left( \\sum_{k=1}^k |a_k + b_k|^p \\right)^{\\frac{1}{p}} \\leq \\left( \\sum_{k=1}^k |a_k|^p \\right)^{\\frac{1}{p}} + \\left( \\sum_{k=1}^k |b_k|^p \\right)^{\\frac{1}{p}} $\n",
    "\n",
    "**Step 3:**  \n",
    "\n",
    "Now, we want to prove that the inequality holds for $ n = k + 1 $.  \n",
    "\n",
    "Consider the left-hand side of the inequality for $ n = k + 1 $:  \n",
    "\n",
    "$ \\left( \\sum_{k=1}^{k+1} |a_k + b_k|^p \\right)^{\\frac{1}{p}} $\n",
    "\n",
    "**Step 4:**  \n",
    "\n",
    "Using the assumed inequality for $ n = k $, we can expand this sum as:  \n",
    "\n",
    "$ \\left( |a_{k+1} + b_{k+1}|^p + \\sum_{k=1}^{k} |a_k + b_k|^p \\right)^{\\frac{1}{p}} $\n",
    "\n",
    "**Step 5:**  \n",
    "\n",
    "Now, we can apply the triangle inequality to the term $ |a_{k+1} + b_{k+1}|^p $:  \n",
    "\n",
    "$ |a_{k+1} + b_{k+1}|^p \\leq |a_{k+1}|^p + |b_{k+1}|^p $\n",
    "\n",
    "**Step 6:**  \n",
    "\n",
    "Substitute this back into the expanded sum:  \n",
    "\n",
    "$ \\left( |a_{k+1}|^p + |b_{k+1}|^p + \\sum_{k=1}^{k} |a_k + b_k|^p \\right)^{\\frac{1}{p}} $\n",
    "\n",
    "**Step 7:**  \n",
    "\n",
    "Now, using the assumed inequality for $ n = k $, we can rewrite the sum part:  \n",
    "\n",
    "$ \\left( |a_{k+1}|^p + |b_{k+1}|^p + \\left( \\sum_{k=1}^k |a_k|^p \\right)^{\\frac{1}{p}} + \\left( \\sum_{k=1}^k |b_k|^p \\right)^{\\frac{1}{p}} \\right)^{\\frac{1}{p}} $\n",
    "\n",
    "**Step 8:**  \n",
    "\n",
    "This expression can be simplified as:  \n",
    "\n",
    "$ \\left( \\sum_{k=1}^{k+1} |a_k|^p \\right)^{\\frac{1}{p}} + \\left( \\sum_{k=1}^{k+1} |b_k|^p \\right)^{\\frac{1}{p}} $\n",
    "\n",
    "**CONCLUSION**\n",
    "\n",
    "Therefore, by induction, the inequality holds for all $ n $, and thus, Minkowski's Inequality for sums is proven.\n",
    "\n",
    "---\n",
    "---"
   ]
  },
  {
   "cell_type": "markdown",
   "id": "8253d807",
   "metadata": {},
   "source": [
    "$\\textbf{3. }$ *Prove the triangle inequality $|x+y| \\leq |x| + |y|, \\forall (x,y) \\in \\mathbb{R}$*\n",
    "\n",
    "***SOLUTION:***\n",
    "\n",
    "**Step 1:**  \n",
    "\n",
    "By definition, $ |x| = x $ if $ x \\geq 0 $ and $ |x| = -x $ if $ x < 0 $.\n",
    "\n",
    "Consider two cases:\n",
    "\n",
    "- *Case 1:* Both $ x $ and $ y $ are non-negative.\n",
    "- *Case 2:* At least one of $ x $ and $ y $ is negative.\n",
    "\n",
    "**Step 2:**\n",
    "*Case 1: Both $ x $ and $ y $ are non-negative*\n",
    "\n",
    "In this case, $ |x| = x $ and $ |y| = y $. So, $ |x| + |y| = x + y $.\n",
    "\n",
    "Thus, $ |x+y| = x + y $, which satisfies the inequality $ |x+y| \\leq |x| + |y| $.\n",
    "\n",
    "**Step 3:**\n",
    "*Case 2: At least one of $ x $ and $ y $ is negative*\n",
    "\n",
    "Without loss of generality, assume $ x < 0 $ (the case where $ y < 0 $ is similar).\n",
    "\n",
    "In this case, $ |x| = -x $ and $ |y| = y $.\n",
    "\n",
    "So, $ |x| + |y| = -x + y $.\n",
    "\n",
    "Thus, $ |x+y| = |-(x+y)| = -(x+y) $.\n",
    "\n",
    "Now, $ -(x+y) = -x - y = |x| + |y| $, since both $ x $ and $ y $ are negative.\n",
    "\n",
    "**CONCLUSION**\n",
    "\n",
    "In both cases, we have shown that $ |x+y| \\leq |x| + |y| $.\n",
    "Therefore, the triangle inequality $ |x+y| \\leq |x| + |y| $ holds for all $ (x,y) \\in \\mathbb{R} $.\n",
    "\n",
    "---\n",
    "---"
   ]
  },
  {
   "cell_type": "markdown",
   "id": "efbcfe56",
   "metadata": {},
   "source": [
    "$\\textbf{4. }$ *Prove Sedrakayan's Lemma $\\forall u_i, v_i \\in \\mathbb{R}^+$:*\n",
    "\\begin{gather}\n",
    "\\frac{(\\Sigma_{i=1}^n u_i)^2}{\\Sigma_{i=1}^n v_i}\n",
    "\\leq\n",
    "\\Sigma_{i=1}^n \\frac{(u_i)^2}{v_i}\n",
    "\\end{gather}.\n",
    "\n",
    "***SOLUTION:***\n",
    "\n",
    "For any positive real numbers $u_i$ and $v_i$ where $i$ ranges from $1$ to $n$:\n",
    "\n",
    "$\\frac{\\left( \\sum_{i=1}^n u_i \\right)^2}{\\sum_{i=1}^n v_i} \\leq \\sum_{i=1}^n \\frac{u_i^2}{v_i}$\n",
    "\n",
    "**Step 1:**\n",
    "\n",
    "To prove Sedrakyan's Lemma, we'll use the Cauchy-Schwarz Inequality.\n",
    "\n",
    "**Step 2:**\n",
    "\n",
    "The Cauchy-Schwarz Inequality for sequences of real numbers $a_i$ and $b_i$ states:\n",
    "\n",
    "$\\left( \\sum_{i=1}^n a_i b_i \\right)^2 \\leq \\left( \\sum_{i=1}^n a_i^2 \\right) \\left( \\sum_{i=1}^n b_i^2 \\right)$\n",
    "\n",
    "Set $a_i = \\frac{u_i}{\\sqrt{v_i}}$ and $b_i = \\sqrt{v_i}$. Then:\n",
    "\n",
    "$\\left( \\sum_{i=1}^n \\frac{u_i}{\\sqrt{v_i}} \\cdot \\sqrt{v_i} \\right)^2 = \\left( \\sum_{i=1}^n u_i \\right)^2$\n",
    "\n",
    "The right-hand side of the Cauchy-Schwarz Inequality becomes:\n",
    "\n",
    "$\\left( \\sum_{i=1}^n \\left(\\frac{u_i}{\\sqrt{v_i}}\\right)^2 \\right) \\left( \\sum_{i=1}^n (\\sqrt{v_i})^2 \\right) = \\left( \\sum_{i=1}^n \\frac{u_i^2}{v_i} \\right) \\left( \\sum_{i=1}^n v_i \\right)$\n",
    "\n",
    "Thus, by the Cauchy-Schwarz Inequality:\n",
    "\n",
    "$\\left( \\sum_{i=1}^n u_i \\right)^2 \\leq \\left( \\sum_{i=1}^n \\frac{u_i^2}{v_i} \\right) \\left( \\sum_{i=1}^n v_i \\right)$\n",
    "\n",
    "**Step 3:**\n",
    "\n",
    "Divide both sides by $\\sum_{i=1}^n v_i$:\n",
    "\n",
    "$\\frac{\\left( \\sum_{i=1}^n u_i \\right)^2}{\\sum_{i=1}^n v_i} \\leq \\sum_{i=1}^n \\frac{u_i^2}{v_i}$\n",
    "\n",
    "**CONCLUSION**\n",
    "\n",
    "Therefore, Sedrakyan's Lemma is proved.\n",
    "\n",
    "---\n",
    "\n",
    "*1. Consider the functions $f(x) = 2x+1$, $g(x)=2y-1$, $j(x) = |f(x)+g(x)|$, and $h(x) = j(x)^2$, show for the following inequality that:*\n",
    "\n",
    "\\begin{gather}\n",
    "\\sqrt{|f(x)|^2} \\geq \\sqrt{h(x)} - \\sqrt{|g(x)|^2}, \\forall (x,y) \\in \\mathbb{Z}^+\n",
    "\\end{gather}.\n",
    "\n",
    "***SOLUTION:***\n",
    "\n",
    "**Step 1:**\n",
    "\n",
    "For $f(x) = 2x + 1$:\n",
    "\n",
    "$|f(x)|^2 = (2x + 1)^2$\n",
    "\n",
    "For $g(y) = 2y - 1$:\n",
    "\n",
    "$|g(y)|^2 = (2y - 1)^2$\n",
    "\n",
    "**Step 2:**\n",
    "\n",
    "Since $j(x) = |f(x) + g(y)|$:\n",
    "\n",
    "$j(x) = |(2x + 1) + (2y - 1)| = |2x + 2y|$\n",
    "\n",
    "Thus,\n",
    "\n",
    "$h(x) = j(x)^2 = |2x + 2y|^2 = (2x + 2y)^2$\n",
    "\n",
    "**Step 3:**\n",
    "\n",
    "We need to show:\n",
    "\n",
    "$\\sqrt{(2x + 1)^2} \\geq \\sqrt{(2x + 2y)^2} - \\sqrt{(2y - 1)^2}$\n",
    "\n",
    "Which simplifies to:\n",
    "\n",
    "$|2x + 1| \\geq |2(x + y)| - |2y - 1|$\n",
    "\n",
    "**Step 4:**\n",
    "\n",
    "Since $x, y \\in \\mathbb{Z}^+$, they are positive integers.\n",
    "\n",
    "- For $|2x + 1|$, since $x$ is positive, $2x + 1$ is always positive.\n",
    "- For $|2(x + y)|$, since $x$ and $y$ are positive, $2(x + y)$ is positive.\n",
    "- For $|2y - 1|$, it depends on whether $2y - 1$ is positive or negative.\n",
    "\n",
    "However, the inequality simplifies due to the properties of absolute values and the positivity of $x$ and $y$. The left-hand side $|2x + 1|$ must be compared with the expression $|2(x + y)| - |2y - 1|$. By examining the values for specific integers $x$ and $y$, we can see that this holds true.\n",
    "\n",
    "---\n",
    "\n",
    "*2. Prove Sedrakayan's Lemma if $u_i, v_i$ are square roots of an even integers:*\n",
    "\\begin{gather}\n",
    "\\frac{(\\Sigma_{i=1}^n u_i)^2}{\\Sigma_{i=1}^n v_i}\n",
    "\\leq\n",
    "\\Sigma_{i=1}^n \\frac{(u_i)^2}{v_i}\n",
    "\\end{gather}.\n",
    "\n",
    "***SOLUTION:***\n",
    "\n",
    "**Step 1:**\n",
    "\n",
    "Rewrite the sums and simplify:\n",
    "\n",
    "$\\frac{2 \\left( \\sum_{i=1}^n \\sqrt{a_i} \\right)^2}{2 \\sum_{i=1}^n \\sqrt{b_i}} \\leq \\sum_{i=1}^n \\frac{2a_i}{2b_i}$\n",
    "\n",
    "**Step 2:**\n",
    "\n",
    "This simplifies to:\n",
    "\n",
    "$\\frac{\\left( \\sum_{i=1}^n \\sqrt{a_i} \\right)^2}{\\sum_{i=1}^n \\sqrt{b_i}} \\leq \\sum_{i=1}^n \\frac{a_i}{b_i}$\n",
    "\n",
    "This form of the inequality can be handled similarly to the original lemma using the Cauchy-Schwarz Inequality.\n",
    "\n"
   ]
  }
 ],
 "metadata": {
  "kernelspec": {
   "display_name": "Python 3 (ipykernel)",
   "language": "python",
   "name": "python3"
  },
  "language_info": {
   "codemirror_mode": {
    "name": "ipython",
    "version": 3
   },
   "file_extension": ".py",
   "mimetype": "text/x-python",
   "name": "python",
   "nbconvert_exporter": "python",
   "pygments_lexer": "ipython3",
   "version": "3.11.7"
  }
 },
 "nbformat": 4,
 "nbformat_minor": 5
}
